Prove special ending lifetime rule for pointer perms

src/LifetimeMemoryPerms.v
@@ -73,25 +73,48 @@ Section Perms.
     eexists. rewrite HPutPut. reflexivity.
   Qed.
 
-  Lemma nonLifetime_ptr p rw o' :
-    @nonLifetime_Perms _ Ss _ ((VPtr p) :: ptr(rw, o', trueP) ▷ tt).
+  Lemma pre_inv_read_perm p v :
+    @pre_inv _ Ss _ (read_perm p v).
+  Proof.
+    repeat intro. cbn. rewrite HGetPut1. auto.
+  Qed.
+  Lemma pre_inv_write_perm p v :
+    @pre_inv _ Ss _ (write_perm p v).
+  Proof.
+    repeat intro. cbn. rewrite HGetPut1. auto.
+  Qed.
+
+  Lemma nonLifetime_ptr {A} p rw o' a (T : VPermType A) (HT : forall xi xs, nonLifetime_Perms (xi :: T ▷ xs)) :
+    @nonLifetime_Perms _ Ss _ ((VPtr p) :: ptr(rw, o', T) ▷ a).
   Proof.
     intros q Hq. destruct p as [b o]. destruct Hq as (? & (v & ?) & ?). subst.
-    destruct H0 as (p & p' & Hp & _ & Hsep & Hlte). destruct rw.
-    - exists (read_perm (b, o + o') v). split; [| split; [| split]].
+    destruct H0 as (p & pt' & Hp & Ht' & Hsep & Hlte).
+    edestruct (HT v a _ Ht') as (pt & Ht & Hlte' & Hnlt & Hguart & Hpret).
+    destruct rw.
+    - assert (Hsep' : (read_perm (b, o + o') v) ⊥ pt).
+      {
+        eapply separate_antimonotone. 2: apply Hlte'.
+        symmetry. eapply separate_antimonotone. 2: apply Hp. symmetry; auto.
+      }
+      exists ((read_perm (b, o + o') v) ** pt). split; [| split; [| split; [| split]]].
       + eexists. split. eexists. reflexivity.
-        cbn. eexists. exists bottom_perm. intuition. reflexivity.
-        apply separate_bottom. rewrite sep_conj_perm_bottom. reflexivity.
-      + etransitivity; eauto. etransitivity; eauto. apply lte_l_sep_conj_perm.
-      + apply nonLifetime_read_perm.
-      + apply guar_inv_read_perm.
-    - exists (write_perm (b, o + o') v). split; [| split; [| split]].
+        cbn. do 2 eexists. split; [| split; [| split]]; eauto; reflexivity.
+      + etransitivity; eauto. apply sep_conj_perm_monotone; auto.
+      + apply nonLifetime_sep_conj_perm; auto. apply nonLifetime_read_perm.
+      + apply guar_inv_sep_conj_perm; auto. apply guar_inv_read_perm.
+      + apply pre_inv_sep_conj_perm; auto. apply pre_inv_read_perm.
+    - assert (Hsep' : (write_perm (b, o + o') v) ⊥ pt).
+      {
+        eapply separate_antimonotone. 2: apply Hlte'.
+        symmetry. eapply separate_antimonotone. 2: apply Hp. symmetry; auto.
+      }
+      exists ((write_perm (b, o + o') v) ** pt). split; [| split; [| split; [| split]]].
       + eexists. split. eexists. reflexivity.
-        cbn. eexists. exists bottom_perm. intuition. reflexivity.
-        apply separate_bottom. rewrite sep_conj_perm_bottom. reflexivity.
-      + etransitivity; eauto. etransitivity; eauto. apply lte_l_sep_conj_perm.
-      + apply nonLifetime_write_perm.
-      + apply guar_inv_write_perm.
+        cbn. do 2 eexists. split; [| split; [| split]]; eauto; reflexivity.
+      + etransitivity; eauto. apply sep_conj_perm_monotone; auto.
+      + apply nonLifetime_sep_conj_perm; auto. apply nonLifetime_write_perm.
+      + apply guar_inv_sep_conj_perm; auto. apply guar_inv_write_perm.
+      + apply pre_inv_sep_conj_perm; auto. apply pre_inv_write_perm.
   Qed.
 
   Lemma separate_write_perm p l v v' :
@@ -108,15 +131,138 @@ Section Perms.
     repeat intro. split; apply H; auto.
   Qed.
 
-  Lemma split_Perms b o l (P Q : @Perms (Si * Ss)) :
-    (VPtr (b, o)) :: ptr(W, 0, trueP) ▷ tt * lowned_Perms' l P Q ⊨
+  Lemma nonLifetime_trueP :
+    forall (xi : Value) (xs : unit), @nonLifetime_Perms _ Ss _ (xi :: trueP ▷ xs).
+  Proof.
+    repeat intro. exists bottom_perm. cbn. intuition.
+    apply bottom_perm_is_bottom.
+    apply nonLifetime_bottom.
+    apply guar_inv_bottom.
+    apply pre_inv_bottom.
+  Qed.
+
+  Lemma nonLifetime_eqp y :
+    forall (xi : Value) (xs : unit), @nonLifetime_Perms _ Ss _ (xi :: eqp y ▷ xs).
+  Proof.
+    repeat intro. exists bottom_perm. cbn. intuition.
+    apply bottom_perm_is_bottom.
+    apply nonLifetime_bottom.
+    apply guar_inv_bottom.
+    apply pre_inv_bottom.
+  Qed.
+
+  Lemma split_Perms_trueP b o l (P Q : @Perms (Si * Ss)) :
+    (VPtr (b, o)) :: ptr(W, 0, trueP) ▷ tt * lowned_Perms l P Q ⊨
       when_Perms l ((VPtr (b, o)) :: ptr(W, 0, trueP) ▷ tt) *
-      lowned_Perms' l
-                    (when_Perms l ((VPtr (b, o)) :: ptr(R, 0, trueP) ▷ tt) * P)
-                    (((VPtr (b, o)) :: ptr(W, 0, trueP) ▷ tt) * Q).
+      lowned_Perms l
+        (when_Perms l ((VPtr (b, o)) :: ptr(R, 0, trueP) ▷ tt) * P)
+        (((VPtr (b, o)) :: ptr(W, 0, trueP) ▷ tt) * Q).
   Proof.
     intros p0 (p' & powned & Hp' & (r1 & r2 & Hr1 & Hr2 & Hr2' & Hsep' & Hr2'' & Hlte' & Hf) & Hsep & Hlte).
-    destruct (nonLifetime_ptr _ _ _ _ Hp') as (p & Hp & Hpp' & Hnlp & Hguarp).
+    destruct (nonLifetime_ptr _ _ _ _ trueP nonLifetime_trueP _ Hp') as (p & Hp & Hpp' & Hnlp & Hguarp & Hprep).
+    exists (when l p Hnlp).
+    assert (Hpr2 : p ⊥ r2).
+    {
+      eapply owned_sep; auto.
+      eapply separate_antimonotone.
+      2: {
+        etransitivity. apply lte_r_sep_conj_perm. eauto.
+      }
+      symmetry. eapply separate_antimonotone; eauto. symmetry. auto.
+    }
+    cbn in Hp.
+    eexists (r1 ** owned l (p ** r2) (nonLifetime_sep_conj_perm _ _ Hnlp Hr2 Hpr2)).
+    split; [| split; [| split]]; auto.
+    - apply when_perm_Perms; auto.
+    - exists r1, (p ** r2), Hr1, (nonLifetime_sep_conj_perm _ _ Hnlp Hr2 Hpr2), (guar_inv_sep_conj_perm _ _ Hguarp Hr2').
+      split; [| split; [| split]].
+      3: reflexivity.
+      {
+        apply sep_owned; auto. eapply separate_antimonotone. 2: apply Hpp'.
+        symmetry. eapply separate_antimonotone. apply Hsep.
+        etransitivity; eauto. apply lte_l_sep_conj_perm.
+      }
+      {
+        apply sep_conj_Perms_perm; auto.
+      }
+      (** Precondition part *)
+      intros p1 (pw & q & (? & (pr & Hpr' & Hpr & ?) & Hlte''') & Hq' & Hsep''' & Hlte'') Hsep''; subst.
+      cbn in Hlte'''.
+      specialize (Hf _ Hq'). destruct Hf as (r & Hr & Hsep_step & Hpre).
+      {
+        symmetry in Hsep''.
+        eapply separate_antimonotone in Hsep''; eauto.
+        eapply separate_antimonotone in Hsep''; eauto.
+        2: apply lte_r_sep_conj_perm.
+        symmetry in Hsep''.
+        eapply separate_antimonotone in Hsep''; eauto.
+        apply sep_conj_perm_monotone. reflexivity.
+        apply owned_monotone. apply lte_r_sep_conj_perm.
+      }
+      destruct Hp as (? & (v & ?) & Hx). subst. rewrite Nat.add_0_r in Hx.
+      rewrite sep_conj_Perms_commut in Hx. rewrite sep_conj_Perms_bottom_identity in Hx.
+      cbn in Hx.
+
+      destruct Hpr as (? & (v' & ?) & Hx'). subst. rewrite Nat.add_0_r in Hx'.
+      rewrite sep_conj_Perms_commut in Hx'. rewrite sep_conj_Perms_bottom_identity in Hx'.
+      cbn in Hx'.
+      exists ((write_perm (b, o) v') ** r). split; [| split].
+      + apply sep_conj_Perms_perm; auto.
+        * cbn. eexists. split. eexists. reflexivity.
+          rewrite Nat.add_0_r.
+          rewrite sep_conj_Perms_commut. rewrite sep_conj_Perms_bottom_identity.
+          cbn. reflexivity.
+        * symmetry. eapply separate_write_perm.
+          apply Hsep_step.
+          eapply separate_antimonotone.
+          2: apply Hx.
+          symmetry. auto.
+      + etransitivity.
+        * apply sep_step_sep_conj_r; eauto. symmetry. auto.
+        * apply sep_step_sep_conj_l; eauto. symmetry. apply Hsep_step. symmetry. auto.
+          eapply sep_step_write_perm.
+          apply sep_step_lte'; eauto.
+      + intros. split; [| split]; auto.
+        * apply Hlte'' in H. destruct H as (? & ? & ?).
+          apply Hlte''' in H. cbn in H.
+          rewrite lGetPut in H. setoid_rewrite nth_error_replace_list_index_eq in H.
+          apply Hx' in H. cbn in *.
+          rewrite HGetPut1 in H |- *; auto. right. reflexivity.
+        * apply Hpre; auto. apply Hlte''; auto.
+        * symmetry. apply Hsep_step.
+          eapply separate_write_perm.
+          eapply separate_antimonotone. symmetry. apply Hpr2. apply Hx.
+    - apply separate_sep_conj_perm.
+      + apply sep_when; auto.
+        symmetry.
+        eapply separate_antimonotone. 2: apply Hpp'.
+        symmetry.
+        eapply separate_antimonotone. apply Hsep. etransitivity; eauto.
+        apply lte_l_sep_conj_perm.
+      + apply when_owned_sep.
+      + symmetry. apply sep_owned; auto. eapply separate_antimonotone. 2: apply Hpp'.
+        symmetry. eapply separate_antimonotone. apply Hsep.
+        etransitivity; eauto. apply lte_l_sep_conj_perm.
+    - etransitivity; eauto.
+      etransitivity. 2: apply sep_conj_perm_monotone; [reflexivity |].
+      2: apply Hlte'.
+      do 2 rewrite <- sep_conj_perm_assoc.
+      do 2 rewrite (sep_conj_perm_commut _ r1).
+      do 2 rewrite sep_conj_perm_assoc.
+      apply sep_conj_perm_monotone; [reflexivity |].
+      etransitivity. apply convert.
+      apply sep_conj_perm_monotone; [| reflexivity]; auto.
+  Qed.
+
+  Lemma split_Perms_eq b o y l (P Q : @Perms (Si * Ss)) :
+    (VPtr (b, o)) :: ptr(W, 0, eqp y) ▷ tt * lowned_Perms l P Q ⊨
+      when_Perms l ((VPtr (b, o)) :: ptr(W, 0, eqp y) ▷ tt) *
+      lowned_Perms l
+        (when_Perms l ((VPtr (b, o)) :: ptr(R, 0, eqp y) ▷ tt) * P)
+        (((VPtr (b, o)) :: ptr(W, 0, eqp y) ▷ tt) * Q).
+  Proof.
+    intros p0 (p' & powned & Hp' & (r1 & r2 & Hr1 & Hr2 & Hr2' & Hsep' & Hr2'' & Hlte' & Hf) & Hsep & Hlte).
+    destruct (nonLifetime_ptr _ _ _ _ (eqp y) (nonLifetime_eqp y) _ Hp') as (p & Hp & Hpp' & Hnlp & Hguarp & Hprep).
     exists (when l p Hnlp).
     assert (Hpr2 : p ⊥ r2).
     {
@@ -141,6 +287,276 @@ Section Perms.
       {
         apply sep_conj_Perms_perm; auto.
       }
+      (** Precondition part *)
+      intros p1 (pw & q & (? & (pr & Hpr' & Hpr & ?) & Hlte''') & Hq' & Hsep''' & Hlte'') Hsep''; subst.
+      cbn in Hlte'''.
+      specialize (Hf _ Hq'). destruct Hf as (r & Hr & Hsep_step & Hpre).
+      {
+        symmetry in Hsep''.
+        eapply separate_antimonotone in Hsep''; eauto.
+        eapply separate_antimonotone in Hsep''; eauto.
+        2: apply lte_r_sep_conj_perm.
+        symmetry in Hsep''.
+        eapply separate_antimonotone in Hsep''; eauto.
+        apply sep_conj_perm_monotone. reflexivity.
+        apply owned_monotone. apply lte_r_sep_conj_perm.
+      }
+      destruct Hp as (? & (v & ?) & Hx). subst. rewrite Nat.add_0_r in Hx.
+      cbn in Hx. destruct Hx as (? & ? & ? & ? & ? & ?). subst.
+      destruct Hpr as (? & (v' & ?) & Hx'). subst. rewrite Nat.add_0_r in Hx'.
+      cbn in Hx'. destruct Hx' as (? & ? & ? & ? & ? & ?). subst.
+      exists ((write_perm (b, o) v') ** r). split; [| split].
+      + apply sep_conj_Perms_perm; auto.
+        * cbn. eexists. split. eexists. reflexivity.
+          rewrite Nat.add_0_r.
+          cbn. do 2 eexists. split; [| split; [| split]].
+          -- reflexivity.
+          -- reflexivity.
+          -- apply separate_bottom.
+          -- rewrite sep_conj_perm_bottom. reflexivity.
+        * symmetry. (* eapply separate_write_perm. *)
+          apply Hsep_step.
+          eapply separate_antimonotone. 2: apply H.
+          eapply separate_antimonotone. 2: apply lte_l_sep_conj_perm.
+          eapply separate_antimonotone. 2: eauto.
+          symmetry. auto.
+      + etransitivity.
+        * apply sep_step_sep_conj_r; eauto. symmetry. auto.
+        * apply sep_step_sep_conj_l; eauto. symmetry. apply Hsep_step. symmetry. auto.
+          apply sep_step_lte'; eauto.
+          etransitivity; eauto.
+          etransitivity; eauto. apply lte_l_sep_conj_perm.
+      + intros. split; [| split]; auto.
+        * apply Hlte'' in H3. destruct H3 as (? & ? & ?).
+          apply Hlte''' in H3. cbn in H3.
+          rewrite lGetPut in H3. setoid_rewrite nth_error_replace_list_index_eq in H3.
+          apply H5 in H3. destruct H3 as (? & ? & ?).
+          apply H0 in H3. cbn in H3. cbn.
+          rewrite HGetPut1 in H3 |- *; auto. right. reflexivity.
+        * apply Hpre; auto. apply Hlte''; auto.
+        * symmetry. apply Hsep_step.
+          eapply separate_antimonotone. 2: apply H.
+          eapply separate_antimonotone. 2: apply lte_l_sep_conj_perm.
+          eapply separate_antimonotone. 2: eauto.
+          symmetry. apply Hpr2.
+    - apply separate_sep_conj_perm.
+      + apply sep_when; auto.
+        symmetry.
+        eapply separate_antimonotone. 2: apply Hpp'.
+        symmetry.
+        eapply separate_antimonotone. apply Hsep. etransitivity; eauto.
+        apply lte_l_sep_conj_perm.
+      + apply when_owned_sep.
+      + symmetry. apply sep_owned; auto. eapply separate_antimonotone. 2: apply Hpp'.
+        symmetry. eapply separate_antimonotone. apply Hsep.
+        etransitivity; eauto. apply lte_l_sep_conj_perm.
+    - etransitivity; eauto.
+      etransitivity. 2: apply sep_conj_perm_monotone; [reflexivity |].
+      2: apply Hlte'.
+      do 2 rewrite <- sep_conj_perm_assoc.
+      do 2 rewrite (sep_conj_perm_commut _ r1).
+      do 2 rewrite sep_conj_perm_assoc.
+      apply sep_conj_perm_monotone; [reflexivity |].
+      etransitivity. apply convert.
+      apply sep_conj_perm_monotone; [| reflexivity]; auto.
+  Qed.
+
+  Definition when_ptr_Perms {A} (l : nat) (rw : RW) (p : Value) (a : A) (T : VPermType A)
+    : @Perms (Si * Ss) :=
+    match p with
+    | VNum _ => top_Perms
+    | VPtr p =>
+        meet_Perms (fun P => exists (v : Value),
+                        P = singleton_Perms
+                              (match rw with
+                               | R => when l (read_perm p v) (nonLifetime_read_perm _ _)
+                               | W => when l (write_perm p v) (nonLifetime_write_perm _ _)
+                               end) *
+                              (v :: T ▷ a))
+    end.
+
+  Definition when_ptr {A} (l : nat) '(rw, o, T) : VPermType A :=
+    {|
+      ptApp := fun x a => when_ptr_Perms l rw (offset x o) a T;
+    |}.
+
+  Definition finished_ptr_Perms {A} (l : nat) (rw : RW) (p : Value) (a : A) (T : VPermType A) : @Perms (Si * Ss) :=
+    match p with
+    | VNum _ => top_Perms
+    | VPtr p =>
+        meet_Perms (fun P => exists (v : Value),
+                        P = singleton_Perms
+                              (match rw with
+                               | R => lfinished l (read_perm p v) (nonLifetime_read_perm _ _)
+                               | W => lfinished l (write_perm p v) (nonLifetime_write_perm _ _)
+                               end) *
+                              (v :: T ▷ a))
+    end.
+
+  Definition finished_ptr {A} (l : nat) '(rw, o, T) : VPermType A :=
+    {|
+      ptApp := fun x a => finished_ptr_Perms l rw (offset x o) a T;
+    |}.
+
+  Lemma typing_end' {A} l b o (T : VPermType A) xs (HT : forall v a, nonLifetime_Perms (v :: T ▷ a)) :
+    typing (specConfig := Ss)
+      ((VPtr (b, o)) :: when_ptr l (W, 0, T) ▷ xs *
+         (lowned_Perms l (when_Perms l ((VPtr (b, o)) :: ptr(R, 0, trueP) ▷ tt))
+            ((VPtr (b, o)) :: ptr(W, 0, trueP) ▷ tt)))
+      (fun _ _ => (VPtr (b, o)) :: finished_ptr l (W, 0, T) ▷ xs)
+      (endLifetime l)
+      (Ret tt).
+  Proof.
+    intros p' c1 c2 (pwt & lowned' & Hpwt & H & Hsep & Hlte) Hpre.
+    destruct Hpwt as (? & (v & ?) & Hpwt); subst.
+    destruct Hpwt as (pwhen & pt & Hpwhen & Hpt & Hsep' & Hlte').
+    destruct (HT _ _ _ Hpt) as (pt' & Hpt' & Hltept' & Hnlpt' & Hguarpt' & Hprept').
+    destruct H as (r1 & r2 & Hr1 & Hr2 & Hr2' & Hsep'' & Hr2'' & Hlte'' & Hf).
+    unfold endLifetime. unfold id.
+    rewritebisim @bind_trigger.
+    pstep. econstructor; eauto; try reflexivity.
+
+    pose proof Hpre as Hpre''.
+    apply Hlte in Hpre. destruct Hpre as (_ & Hpre & _).
+    apply Hlte'' in Hpre. destruct Hpre as (_ & H & _).
+    cbn in H. setoid_rewrite H.
+    rewritebisim @bind_trigger.
+    specialize (Hf (when l (write_perm (b, o + 0) v) (nonLifetime_write_perm (b, o + 0) v))).
+    destruct Hf as (q & Hq & Hsep_step & Hpre).
+    {
+      apply when_perm_Perms. eexists. split. eexists. reflexivity. cbn.
+      do 2 eexists. split; [| split; [| split]]. 2: auto.
+      - apply read_lte_write.
+      - apply separate_bottom.
+      - rewrite sep_conj_perm_bottom. reflexivity.
+    }
+    {
+      apply Hlte in Hpre''. destruct Hpre'' as (? & ? & ?).
+      eapply separate_antimonotone; eauto.
+      symmetry. eapply separate_antimonotone; eauto.
+      eapply separate_antimonotone; eauto. symmetry. eauto.
+      etransitivity; eauto. apply lte_l_sep_conj_perm.
+    }
+    destruct Hq as (? & (v' & ?) & Hq); subst.
+    rewrite sep_conj_Perms_commut in Hq. rewrite sep_conj_Perms_bottom_identity in Hq.
+    cbn in Hq.
+    assert (Hv: Some v = read (lget c1) (b, o + 0)).
+    {
+      apply Hlte in Hpre''. destruct Hpre'' as (Hpre'' & _).
+      apply Hlte' in Hpre''. destruct Hpre'' as (Hpre'' & _).
+      apply Hpwhen in Hpre''. cbn in Hpre''. auto.
+    }
+    assert (v = v'). {
+      specialize (Hpre c1 c2).
+      apply Hq in Hpre.
+      - (* from this we can get that (b, o) points to v using pwhen *)
+        cbn in Hpre.
+        rewrite HGetPut1 in Hpre. rewrite <- Hv in Hpre. inversion Hpre. auto.
+      - rewrite replace_list_index_eq; auto. rewrite lPutGet. cbn.
+        intros. apply Hv.
+      - apply Hlte''. apply Hlte. rewrite replace_list_index_eq; auto.
+        rewrite lPutGet. auto.
+    } subst. rename v' into v.
+    assert (Hsep''': owned l r2 Hr2 ⊥ pt'). {
+      eapply separate_antimonotone; eauto.
+      eapply separate_antimonotone. 2: apply lte_r_sep_conj_perm.
+      eapply separate_antimonotone; eauto.
+      symmetry.
+      eapply separate_antimonotone; eauto.
+      etransitivity; eauto. apply lte_r_sep_conj_perm.
+    }
+    econstructor; unfold id; auto.
+    {
+      cbn in *. apply Hlte. constructor 1. right.
+      apply Hlte''. constructor 1. right. right.
+      repeat rewrite lGetPut.
+      split; [| split; [| split]].
+      - intros. apply nth_error_replace_list_index_neq; auto.
+        apply nth_error_Some. intro.
+        unfold statusOf, Lifetimes in H. rewrite H1 in H. inversion H.
+      - apply replace_list_index_length; auto. apply nth_error_Some. intro.
+        unfold statusOf, Lifetimes in H. rewrite H0 in H. inversion H.
+      - unfold statusOf. apply nth_error_replace_list_index_eq.
+      - rewrite lPutPut, replace_list_index_twice. reflexivity.
+    }
+    2: {
+      econstructor.
+      2: {
+        cbn. eexists. split. eexists. reflexivity. cbn.
+        eexists (lfinished l q _). exists pt'. split; [| split; [| split]].
+        - apply lfinished_monotone; eauto.
+        - auto.
+        - apply lfinished_separate'; auto.
+          apply Hsep_step. symmetry. eapply owned_sep; eauto. symmetry. eauto.
+        - reflexivity.
+      }
+      cbn. rewrite lGetPut.
+      split; split.
+      - symmetry. apply nth_error_replace_list_index_eq.
+      - apply Hpre.
+        + cbn. rewrite lGetPut. rewrite HGetPut1.
+          intros. apply Hv.
+        + rewrite replace_list_index_eq; auto.
+          rewrite lPutGet.
+          apply Hlte''. apply Hlte. auto.
+      - apply Hprept'. apply Hltept'. apply Hlte'. apply Hlte; auto.
+      - apply lfinished_separate'; auto.
+        apply Hsep_step. symmetry. eapply owned_sep; eauto. symmetry. eauto.
+    }
+    eapply sep_step_lte; eauto.
+    rewrite sep_conj_perm_commut.
+    eapply sep_step_lte. apply sep_conj_perm_monotone. eauto.
+    etransitivity. 2: apply Hlte'. etransitivity. 2: apply lte_r_sep_conj_perm.
+    apply Hltept'.
+    eapply sep_step_lte.
+    rewrite sep_conj_perm_assoc. apply lte_r_sep_conj_perm.
+    apply sep_step_sep_conj_l; auto.
+    etransitivity. 2: eapply sep_step_owned_finished.
+    apply owned_sep_step; auto.
+
+    Unshelve.
+    eapply nonLifetime_sep_step. 2: eauto. auto.
+  Qed.
+
+
+  Lemma split_Perms' b o l (P Q : @Perms (Si * Ss)) T (xs : Ss)
+    (HT : forall xi xs, nonLifetime_Perms (xi :: T ▷ xs)) :
+    (VPtr (b, o)) :: ptr(W, 0, T) ▷ xs * lowned_Perms l P Q ⊨
+      (VPtr (b, o)) :: when_ptr l (W, 0, T) ▷ xs *
+      lowned_Perms l
+        ((VPtr (b, o)) :: when_ptr l (R, 0, trueP) ▷ xs * P)
+        ((VPtr (b, o)) :: when_ptr l (W, 0, trueP) ▷ xs * Q).
+  Proof.
+    intros p0 (p' & powned & Hp' & (r1 & r2 & Hr1 & Hr2 & Hr2' & Hsep' & Hr2'' & Hlte' & Hf) & Hsep & Hlte).
+    destruct (nonLifetime_ptr _ _ _ _ T HT _ Hp') as (p'' & Hp'' & Hpp' & Hnlp & Hguarp).
+    destruct Hp'' as (? & (v & ?) & Hasdf). subst.
+    destruct Hasdf as (p & pt & Hp & Hpt & Hsep'' & Hlte'').
+    cbn in Hp.
+    exists (when l p'' Hnlp).
+    assert (Hpr2 : p ⊥ r2).
+    {
+      eapply owned_sep; auto.
+      eapply separate_antimonotone.
+      2: {
+        etransitivity. apply lte_r_sep_conj_perm. eauto.
+      }
+      symmetry. eapply separate_antimonotone; eauto. symmetry. auto.
+    }
+    eexists (r1 ** owned l (p ** r2) (nonLifetime_sep_conj_perm _ _ Hnlp Hr2 Hpr2)).
+    split; [| split; [| split]]; auto.
+    - apply when_perm_Perms; auto.
+    - exists r1, (p ** r2), Hr1, (nonLifetime_sep_conj_perm _ _ Hnlp Hr2 Hpr2), (guar_inv_sep_conj_perm _ _ Hguarp Hr2').
+      split; [| split; [| split]].
+      3: reflexivity.
+      {
+        apply sep_owned; auto. eapply separate_antimonotone. 2: apply Hpp'.
+        symmetry. eapply separate_antimonotone. apply Hsep.
+        etransitivity; eauto. apply lte_l_sep_conj_perm.
+      }
+      {
+        apply sep_conj_Perms_perm; auto.
+      }
+      (** Precondition part *)
       intros p1 (pw & q & (? & (pr & Hpr' & Hpr & ?) & Hlte''') & Hq' & Hsep''' & Hlte'') Hsep''; subst.
       cbn in Hlte'''.
       specialize (Hf _ Hq'). destruct Hf as (r & Hr & Hsep_step & Hpre).
@@ -209,3 +625,4 @@ Section Perms.
       etransitivity. apply convert.
       apply sep_conj_perm_monotone; [| reflexivity]; auto.
   Qed.
+End Perms.
